
\documentclass[a4paper,10pt]{article}

\usepackage[
	left=1cm,right=1cm,top=1cm,bottom=2cm,
    papersize={250mm,350mm}
]{geometry}


\usepackage[english]{babel}
\usepackage[utf8]{inputenc}

\usepackage{amsmath}
\usepackage{amssymb}

\usepackage{physics}

\usepackage{verbatim}

\usepackage[squaren]{SIunits}
\usepackage{graphicx}
\usepackage{xcolor}

\newcommand{\mi}{\mathrm{i}}
\newcommand{\suml}{\sum\limits}
\newcommand{\prodl}{\prod\limits}
\newcommand{\intl}{\int\limits}


\begin{document}

\paragraph{Parameters}

\begin{align}
	a&>0
\\
	b&>0
\\
	K&\geq 0
\\
	D_0
	&\geq 0
\\
	\tau
	&\geq 0
\end{align}


\paragraph{Potential}

\begin{align}
	V(x)
	&=
	\frac{a}{4}
	x^4
	-
	\frac{b}{2}
	x^2
	=
	\frac{a}{4}
	x^2
	\pqty{
		x-\sqrt{\frac{2b}{a}}
	}
	\pqty{
		x+\sqrt{\frac{2b}{a}}	
	}
\end{align}

\paragraph{Force}

\begin{align}
	F(x)
	&=
	-\pdv{V}{x}
	=
	-
	a
	x^3
	+
	b
	x
\end{align}


We have 2 Hypervolumes

\begin{align}
	\mathcal{V}_t
	&\subset
	\mathbb{R}^{n_t}
\\
	\mathcal{V}_\tau
	&\subset
	\mathbb{R}^{n_\tau}
\\
	\mathcal{V}
	&=
	\mathcal{V}_t
	\times
	\mathcal{V}_\tau
\\
	n_t
	&\geq
	n_\tau
\end{align}


\begin{align}
	\dot{X_t}
	&=
	F(X,X_\tau)
	\dd{t}
	+
	\sqrt{2D_0}
	\dd{B}_t
\\	
	&=
	-
	a
	X_t^3
	\dd{t}
	+
	b
	X_t
	\dd{t}
	+
	K
	(X_t-X_\tau)
	\dd{t}
	+
	\sqrt{2D_0}
	\dd{B}_t
\end{align}

\begin{align}
	F(x,x_\tau)
	&=
	F_1(x)
	+
	F_2(x_\tau)
	=
	-
	ax^3
	+
	(b+K)x
	-
	Kx_\tau
\end{align}

\begin{align}
	\pdv{t}
	\rho_1
	&=
	-
	\pdv{x}
	\intl_{\mathcal{V}_\tau}
	\dd{x_\tau}
	F(x,x_\tau)
	\rho_2
	(x,t;x_\tau,t-\tau)
	+
	D_0
	\pdv[2]{x}
	\rho_1(x,t)
\\
	&=
	-
	\pdv{x}
	F_1(x)
	\intl_{\mathcal{V}_\tau}
	\dd{x_\tau}
	\rho_2
	(x,t;x_\tau,t-\tau)
	-
	\pdv{x}
	\intl_{\mathcal{V}_\tau}
	\dd{x_\tau}
	F_2(x_\tau)
	\rho_2
	(x,t;x_\tau,t-\tau)	
	+
	D_0
	\pdv[2]{x}
	\rho_1(x,t)
\\
	&=
	-
	\pdv{x}
	F_1(x)
	\rho_1
	(x,t)
	-
	\pdv{x}
	\intl_{\mathcal{V}_\tau}
	\dd{x_\tau}
	F_2(x_\tau)
	\rho_2
	(x,t;x_\tau,t-\tau)	
	+
	D_0
	\pdv[2]{x}
	\rho_1(x,t)
\end{align}

\begin{align}
	\pdv{t}
	\rho_1
	&=
	-\left( 
	\pdv{F_1}{x}
	\rho_1
	(x,t)
	-
	F_1(x)
	\pdv{x}
	\rho_1
	(x,t)
	-
	\pdv{x}
	\intl_{\mathcal{V}_\tau}
	\dd{x_\tau}
	F_2(x_\tau)
	\rho_2
	(x,t;x_\tau,t-\tau)	
	+
	D_0
	\pdv[2]{x}
	\rho_1(x,t)
\end{align}


\begin{align}
	\pdv{t}
	\rho_2
	&=
	-
	\pdv{x}
	F(x,x_\tau)
	\rho_2
	(x,t;x_\tau,t-\tau)
	+
	D_0
	\pdv[2]{x}
	\rho_2
	(x,t;x_\tau,t-\tau)
	+
	\pdv{x_\tau}
	\rho_2
	(x,t;x_\tau,t-\tau)
	\intl_{\mathcal{V}_t}
	\dd{\dot{x}_\tau}
	\rho_1
	(\dot{x}_\tau,t-\tau)
	\dot{x}_\tau
\\
	&=
	-
	\pdv{x}
	F(x,x_\tau)
	\rho_2
	(x,t;x_\tau,t-\tau)
	+
	D_0
	\pdv[2]{x}
	\rho_2
	(x,t;x_\tau,t-\tau)
	+
	\pdv{x_\tau}
	\rho_2
	(x,t;x_\tau,t-\tau)
	\pqty{
		\intl_{\mathcal{V}_t}
		\dd{\dot{x}_\tau}
		\rho_1
		(\dot{x}_\tau,t-\tau)
		\dot{x}_\tau
	}
\\
	&=
	-
	\pdv{x}
	F_1(x)
	\rho_2
	(x,t;x_\tau,t-\tau)
	-
	F_2(x_\tau)
	\pdv{x}
	\rho_2
	(x,t;x_\tau,t-\tau)
	+
	D_0
	\pdv[2]{x}
	\rho_2
	(x,t;x_\tau,t-\tau)
	+
	\pdv{x_\tau}
	\rho_2
	(x,t;x_\tau,t-\tau)
	\pqty{
		\intl_{\mathcal{V}_t}
		\dd{\dot{x}_\tau}
		\rho_1
		(\dot{x}_\tau,t-\tau)
		\dot{x}_\tau
	}
\end{align}

\begin{align}
	\pdv{f}{x}
	&\sim
	\frac{f(x_{i+1})-f(x_{i-1})}{2\Delta x}
\\
	\pdv[2]{f}{x}
	&\sim
	\frac{2f(x_{i})-f(x_{i-1})-f(x_{i+1})}{\Delta x^2}
\end{align}

\begin{align}
	\intl_{\mathcal{V}}
	\dd{x}
	f(x)
	&=
	\Delta x
	\suml_{i=1}^{N_\mathcal{V}}
	f(x_i)
\end{align}


\begin{comment}


\begin{align}
	f(\vb{x})
	&=
	-ax_1^3
	+\beta x_1
	-
	K
	x_2
\\
	&=
	f_1(x_1)
	+
	f_2(x_2)
\end{align}

\begin{align}
	\pdv{t}
	\rho_1
	(x_1,t)
	&=
	-
	f_1^\prime(x_1)
	\rho_1
	(x_1,t)
	-
	f_1(x_1)
	\pdv{x_1}	
	\rho_1
	(x_1,t)
	-
	\intl
	\dd{x_2}
	f_2(x_2)
	\pdv{x_1}
	\rho_2
	(\vb{x},t)
	+
	D_0
	\pdv[2]{x_1}
	\rho_1
	(x_1,t)
\\
	\pdv{t}
	\rho_2
	(\vb{x},t)
	&=
	-
	f_1^\prime(x_1)
	\rho_2
	(\vb{x},t)
	-
	f(x_1)
	\pdv{x_1}
	\rho_2
	(\vb{x},t)
	-
	f(x_2)
	\pdv{x_1}
	\rho_2
	(\vb{x},t)
	+
	D_0
	\pdv[2]{x_1}
	\rho_2
	(\vb{x},t)
	+
	\pdv{x_2}
	\pqty{
		\intl
		\dd{v_2}
		\rho_1(v_2,t-\tau)
		v_2
	}
	\rho_2(\vb{x},t)
\end{align}

\begin{align}
	\pdv{t}
	\vb*{\rho}
	(\vb{x},t)
	&=
	-
	f_1^\prime
	(x_1)
	\vb*{\rho}
	(\vb{x},t)
	-
	f_1
	(x_1)
	\pdv{x_1}	
	\vb*{\rho}
	(\vb{x},t)
	-
	\vb{e}_2
	\cdot
	f_2(x_2)
	\pdv{x_1}
	\vb*{\rho}
	(\vb{x},t)
	+
	D_0
	\pdv[2]{x_1}
	\vb*{\rho}
	(\vb{x},t)
	+
	\pmqty{
		-
		\pdv{x_1}
		\intl\dd{x_2}
		f_2(x_2)
		\rho_2
		(\vb{x},t)
		\\
		\pdv{x_2}
		\intl\dd{v_2}
		v_2
		\rho_1(v_2,t-\tau)
		\rho_2
		(\vb{x},t)
	}
\end{align}

\end{comment}

\end{document}