\documentclass[a4paper,10pt]{article}

\usepackage[
	left=1cm,right=1cm,top=1cm,bottom=2cm,
    papersize={250mm,350mm}
]{geometry}


\usepackage[english]{babel}
\usepackage[utf8]{inputenc}

\usepackage{amsmath}
\usepackage{amssymb}

\usepackage{physics}

\usepackage{verbatim}

\usepackage[squaren]{SIunits}
\usepackage{graphicx}
\usepackage{xcolor}

\newcommand{\mi}{\mathrm{i}}
\newcommand{\suml}{\sum\limits}
\newcommand{\prodl}{\prod\limits}
\newcommand{\intl}{\int\limits}

\setlength{\parindent}{0pt}

\DeclareMathAlphabet\mathbfcal{OMS}{cmsy}{b}{n}

\begin{document}

\begin{align}
	F
	&=
	m_0\ddot{x}
\end{align}

\begin{align}
	F
	&=
	F_0(x)
	+
	F_1
\end{align}

\begin{align}
	F_0(x)
	&=
	-\pdv{V_0}{x}
\end{align}

\begin{align}
	F_\gamma
	(\dot{x})
	&=
	-\gamma
	\dot{x}
\end{align}

\begin{align}
	F_0(x)
	+
	F_\gamma
	(\dot{x})
	+
	F_2
	&=
	m_0
	\ddot{x}
\end{align}

\begin{align}
	\frac{m_0}{\gamma}
	\ddot{x}
	+
	\dot{x}
	&=
	\gamma^{-1}
	F_0(x)
	+
	\gamma^{-1}
	F_2
\end{align}


\begin{align}
	\dot{x}
	&=
	F_0(x)
	+
	F_2
\end{align}


\begin{align}
	V_0
	(x)
	&=
	\frac{a}{4}
	x^4
	-
	\frac{b}{2}
	x^2
	+
	\frac{b^2}{4a}
\\
	&=
	\frac{a}{4}
	x^2
	\pqty{
		x-\sqrt{\frac{2b}{a}}
	}
	\pqty{
		x+\sqrt{\frac{2b}{a}}	
	}
	+
	\frac{b^2}{4a}
\end{align}

\begin{align}
	a,b&>0
\end{align}

\begin{align}
	F_0(x)
	&=
	-ax^3
	+bx
\end{align}

\begin{align}
	F_\xi(t)
	&=
	\sqrt{2D_0}
	\xi(t)
\end{align}

\begin{align}
	\expval{\xi(t)}
	&=
	0,
	\quad
	\expval{\xi(t)\xi(t^\prime)}
	=
	\delta(t-t^\prime)
\end{align}

\begin{align}
	\dot{X}
	&=
	F_0(X)
	+
	F_\xi(t)
\\
	&=
	-aX^3+bX
	\sqrt{2D_0}
	\xi(t)
\end{align}

\begin{align}
	\partial_t
	\varrho
	&=
	-
	\partial_x
	F_0(x)
	\varrho(x,t)
	+
	D_0
	\partial_x^2
	\varrho(x,t)
\end{align}

\begin{align}
	\partial_t
	\varrho
	-
	\partial_x
	\pqty{
		-
		F_0(x)
		\varrho(x,t)
		+
		D_0
		\partial_x
		\varrho(x,t)
	}
	&=
	0
\end{align}

\begin{align}
	\partial_t
	\varrho
	-
	\partial_x
	\pqty{
		(ax^3-bx)
		\varrho(x,t)
		+
		D_0
		\partial_x
		\varrho(x,t)
	}
	&=
	0
\end{align}

\begin{align}
	F_\tau
	(x,x_\tau)
	&=
	Kx
	-
	Kx_\tau
\end{align}

\begin{align}
	\dot{X}
	&=
	F_0(X)
	+
	F_\tau(X,X_\tau)
	+
	F_\xi(t)
	\\
	&=
	-aX^3
	+
	(b+K)
	X
	-
	KX_\tau
	+
	\sqrt{2D_0}
	\xi(t)
\\
	&=
	F_0^\prime(X)
	+
	F_\tau^\prime(X_\tau)
	+
	\sqrt{2D_0}
	\xi(t)
\end{align}
















\end{document}